src/Narcissus/Formats/Label.v
@@ -1,0 +1,91 @@
+Require Import
+        Fiat.Common
+        Fiat.Computation
+        Fiat.Computation.Notations
+        Fiat.Narcissus.Common.Specs
+        Fiat.Narcissus.Common.WordFacts
+        Fiat.Narcissus.BaseFormats.
+
+
+Unset Implicit Arguments.
+
+Require Import Strings.String. (* For errors*)
+
+(*** TAGS/ LABELS
+     TOD: Move to other file
+ **)
+  Definition format_label {T B C} (label: string): @FormatM T B C -> @FormatM T B C := id.
+  Lemma format_label_equiv: forall S T C label format,
+      @EquivFormat S T C (format_label label format) format.
+  Proof.
+    intros. constructor; simpl; unfold format_label, id; simpl; intros ? **; auto.
+  Qed.
+
+
+(** END OF TAGS/LABELS
+ **)
+
+
+Require Import Fiat.Narcissus.BinLib.AlignedByteString.
+Require Import Strings.String. (* For errors*)
+Require Import Fiat.Narcissus.Stores.EmptyStore.
+
+Definition encoder_tag {CacheFormat S} (label: string)
+           (encoder: forall n,  (*@AlignedEncodeM c S sz*)
+                      ByteBuffer.t n -> nat -> S -> CacheFormat -> Hopefully (ByteBuffer.t n * nat * CacheFormat)):
+  (*@AlignedEncodeM c S sz*)
+                   forall n, ByteBuffer.t n -> nat -> S -> CacheFormat -> Hopefully (ByteBuffer.t n * nat * CacheFormat):=
+    fun C S n s c => catchError (encoder C S n s c) (LabelError label).
+Definition decoder_tag {BS CD A} (label: string)
+           (decoder: BS ->
+                     CD ->
+                     Hopefully (A * BS * CD)):
+  BS -> CD -> Hopefully (A * BS * CD):= 
+  fun b s  => catchError (decoder b s) (LabelError label).
+Definition aligned_decoder_tag {BS CD A} (label: string)
+           (decoder: BS ->
+                     CD ->
+                     Hopefully (A * BS * CD)):
+  BS -> CD -> Hopefully (A * BS * CD):= 
+  fun b s  => catchError (decoder b s) (LabelError label).
+
+Lemma tag_decode_simple_correct
+  : forall A tag
+           (format_A : A ->
+                       CacheFormat -> Comp (ByteString * CacheFormat))
+           (A_cache_inv : CacheDecode -> Prop),
+  forall
+    (decode_A : ByteString ->
+                CacheDecode ->
+                Hopefully (A * ByteString * CacheDecode))
+    (A_predicate : A -> Prop),
+    CorrectDecoder ByteStringQueueMonoid A_predicate A_predicate eq
+                   format_A decode_A A_cache_inv format_A ->
+    CorrectDecoder ByteStringQueueMonoid A_predicate A_predicate eq
+                   (format_label tag format_A)
+                   (decoder_tag tag decode_A)
+                   A_cache_inv
+                   (format_label tag format_A).
+Proof.
+  unfold format_label, id; simpl; intros.
+  (* PROOF SKETCH: `format_label` and `decoder_tag` are computational irrelevant.
+     Proof technique: Prove an equivalence relation for `decoder_tag` and a morphism for `CorrectDecoder`
+   *)
+Admitted.
+
+Lemma EquivFormat_label: forall S T C label format format',
+    @EquivFormat S T C format format' ->
+    @EquivFormat S T C (format_label label format) (format_label label format').
+Proof. unfold format_label, id; auto. Qed.
+(** END MOVE
+ **)
+
+
+
+(** end move
+*)
+
+(* From now on to deal with format_label you must use the lemmas in
+this file. This is important so automation doens't just unfold and
+simplify it away.  *)
+Opaque format_label.
